Формулировка:
```spoiler-markdown
Пусть $f(x)$ - дифференцируема в $x_{0}$, $g(y)$ - дифференцируема в $y_{0} = f(x_{0})$, тогда:
$h(x) = g(f(x))$ - дифференцируема в $x_{0}$ и $h'(x) = g'(f(x_{0})) \cdot f'(x_{0})$
```

Д-во:
```spoiler-markdown
$$\Delta y = f(x_{0} + \Delta x) - f(x_{0}) = f'(x_{0})\Delta x + o(\Delta x)$$
$$\Delta g = g'(y_{0})\Delta y + o(\Delta y) = g'(y_{0})(f'(x_{0})\Delta x + o(\Delta x)) + o(\Delta y) =$$
$$= \underbrace{g'(y_{0})f'(x_{0})}_{h'(x)}\Delta x + \underbrace{ \underbrace{ g'(y_{0})o(\Delta x) }_{o(\Delta x)} + \underbrace{ o(\Delta y) }_{o(\Delta x)} }_{ o(\Delta x) } = \Delta h ~~~\square$$
Примечание:
Через определение доказывать не стоит, так как $f(x) - f(x_{0})$ может быть $=0$
```