Формулировка:
```spoiler-markdown
Для любого $n \in \mathbb{N}$:
$$(\cos\varphi+i\sin\varphi)^{n}=\cos n\varphi+i\sin n\varphi$$
```

Д-во:
```spoiler-markdown
По индукции.

База индукции очевидна.

Шаг индукции:
Пусть $(\cos\varphi + i\sin\varphi)^{k-1} = \cos((k-1)\varphi) + i\sin((k-1)\varphi)$.
Тогда:
$$\begin{align}
(\cos\varphi + i\sin\varphi)^{k} &= (\cos\varphi + i\sin\varphi)^{k-1} \cdot (\cos\varphi + i\sin\varphi) = \\
&= (\cos((k-1)\varphi) + i\sin((k-1)\varphi)) \cdot (\cos\varphi + i\sin\varphi) \\
&= \cos(k\varphi) + i\sin(k\varphi)
\end{align}$$
$\square$
```