Формулировка:
```spoiler-markdown
Пусть $f(x)$ - дифференцируема $n$ раз и для простоты доказательства $f^{(n)}(x)$ - непрерывна в $x_{0}$. Тогда:
$$f(x) = \sum_{k=0}^{n}\dfrac{f^{(k)}(x_{0})}{k!}(x-x_{0})^{k} + o((x-x_{0})^{n})$$
```

Д-во:
```spoiler-markdown
Из непрерывности: ${} f^{(n)}(x) = f^{(n)}(x_{0}) + o(1),~ (x \to x_{0}) {}$. Тогда:
$$f(x) = \sum_{k=0}^{n-1}\dfrac{f^{(k)}(x_{0})}{k!}(x-x_{0})^{k} + \dfrac{f^{(n)}(x_{0}) + o(1)}{n!}(x-x_{0})^{n} = \sum_{k=0}^{n}\dfrac{f^{(k)}(x_{0})}{k!}(x-x_{0})^{k} + o((x-x_{0})^{n}) ~~~\square$$
```
