Формулировка:
```spoiler-markdown
$\lim_{n \to \infty} a_{n} = a,~~ \lim_{n \to \infty} b_{n} = b,~~ b \neq 0 \Rightarrow \lim_{n \to \infty} \left(\dfrac{a_{n}}{b_{n}}\right) = \dfrac{a}{b}$
```

Д-во:
```spoiler-markdown
Докажем, что $\lim_{n \to \infty} \dfrac{1}{b_{n}} = \dfrac{1}{b}$: ($n > N_{1}$)
По определению: $\forall{\epsilon > 0}~~ \exists{N_{2}}~~ \forall{n>N_{2}}~~ |b_{n} - b| < \dfrac{\epsilon|b|^{2}}{2}$, тогда:
$$|\dfrac{1}{b_{n}} - \dfrac{1}{b}| = | \dfrac{b_{n}-b}{b_{n}b} | < \dfrac{|b_{n}-b|}{\dfrac{|b|}{2}|b|}~~ (по~~лемме~~об~~отделимости~~от~~0)~~ <  \dfrac{\dfrac{\epsilon|b|^{2}}{2}}{\dfrac{|b|^{2}}{2}} = \epsilon$$
Тогда: $\lim_{n \to \infty} \dfrac{a_{n}}{b_{n}} = \lim_{n \to \infty} \left(a_{n} \cdot \dfrac{1}{b_{n}}\right) = a \cdot \dfrac{1}{b} = \dfrac{a}{b}~~~ \square$
```
